disk-betree/ImplModelSplit.i.dfy
@@ -1,0 +1,453 @@
+include "ImplModelCache.i.dfy"
+
+module ImplModelSplit { 
+  import opened ImplModel
+  import opened ImplModelIO
+  import opened ImplModelCache
+
+  import opened Options
+  import opened Maps
+  import opened Sequences
+  import opened Sets
+
+  import opened BucketsLib
+  import PivotsLib
+
+  import opened NativeTypes
+
+  function {:opaque} CutoffNodeAndKeepLeft(node: Node, pivot: Key) : (node': Node)
+  requires WFNode(node)
+  ensures |node'.buckets| == |node'.pivotTable| + 1
+  ensures node'.children.Some? ==> |node'.buckets| == |node'.children.value|
+  {
+    var cLeft := Pivots.CutoffForLeft(node.pivotTable, pivot);
+    var leftPivots := node.pivotTable[.. cLeft];
+    var leftChildren := if node.children.Some? then Some(node.children.value[.. cLeft + 1]) else None;
+    var splitBucket := KMTable.splitLeft(node.buckets[cLeft], pivot);
+    var leftBuckets := node.buckets[.. cLeft] + [splitBucket];
+    Node(leftPivots, leftChildren, leftBuckets)
+  }
+
+  lemma CutoffNodeAndKeepLeftCorrect(node: Node, pivot: Key)
+  requires WFNode(node)
+  requires BT.WFNode(INode(node))
+  ensures var node' := CutoffNodeAndKeepLeft(node, pivot);
+    && WFNode(node')
+    && INode(node') == BT.CutoffNodeAndKeepLeft(INode(node), pivot)
+  {
+    reveal_CutoffNodeAndKeepLeft();
+    BT.reveal_CutoffNodeAndKeepLeft();
+    var cLeft := Pivots.CutoffForLeft(node.pivotTable, pivot);
+    var leftPivots := node.pivotTable[.. cLeft];
+    var leftChildren := if node.children.Some? then Some(node.children.value[.. cLeft + 1]) else None;
+    var splitBucket := KMTable.splitLeft(node.buckets[cLeft], pivot);
+    KMTable.splitLeftCorrect(node.buckets[cLeft], pivot);
+    var leftBuckets := node.buckets[.. cLeft] + [splitBucket];
+    Pivots.WFSlice(node.pivotTable, 0, cLeft);
+    KMTable.Islice(node.buckets, 0, cLeft);
+    KMTable.IPopBack(node.buckets[.. cLeft], splitBucket);
+    WFSplitBucketListLeft(KMTable.ISeq(node.buckets), node.pivotTable, cLeft, pivot);
+  }
+
+  function {:opaque} CutoffNodeAndKeepRight(node: Node, pivot: Key)
+  : (node': Node)
+  requires WFNode(node)
+  ensures |node'.buckets| == |node'.pivotTable| + 1
+  ensures node'.children.Some? ==> |node'.buckets| == |node'.children.value|
+  {
+    var cRight := Pivots.CutoffForRight(node.pivotTable, pivot);
+    var rightPivots := node.pivotTable[cRight ..];
+    var rightChildren := if node.children.Some? then Some(node.children.value[cRight ..]) else None;
+    var splitBucket := KMTable.splitRight(node.buckets[cRight], pivot);
+    var rightBuckets := [splitBucket] + node.buckets[cRight + 1 ..];
+    Node(rightPivots, rightChildren, rightBuckets)
+  }
+
+  lemma CutoffNodeAndKeepRightCorrect(node: Node, pivot: Key)
+  requires WFNode(node)
+  requires BT.WFNode(INode(node))
+  ensures var node' := CutoffNodeAndKeepRight(node, pivot);
+    && WFNode(node')
+    && INode(node') == BT.CutoffNodeAndKeepRight(INode(node), pivot)
+  {
+    reveal_CutoffNodeAndKeepRight();
+    BT.reveal_CutoffNodeAndKeepRight();
+    var cRight := Pivots.CutoffForRight(node.pivotTable, pivot);
+    var rightPivots := node.pivotTable[cRight ..];
+    var rightChildren := if node.children.Some? then Some(node.children.value[cRight ..]) else None;
+    var splitBucket := KMTable.splitRight(node.buckets[cRight], pivot);
+    KMTable.splitRightCorrect(node.buckets[cRight], pivot);
+    var rightBuckets := [splitBucket] + node.buckets[cRight + 1 ..];
+    Pivots.WFSuffix(node.pivotTable, cRight);
+    KMTable.Isuffix(node.buckets, cRight + 1);
+    KMTable.IPopFront(splitBucket, node.buckets[cRight + 1 ..]);
+    WFSplitBucketListRight(KMTable.ISeq(node.buckets), node.pivotTable, cRight, pivot);
+  }
+
+  function {:opaque} CutoffNode(node: Node, lbound: Option<Key>, rbound: Option<Key>)
+  : (node' : Node)
+  requires WFNode(node)
+  ensures |node'.buckets| == |node'.pivotTable| + 1
+  ensures node'.children.Some? ==> |node'.buckets| == |node'.children.value|
+  {
+    match lbound {
+      case None => (
+        match rbound {
+          case None => (
+            node
+          )
+          case Some(rbound) => (
+            CutoffNodeAndKeepLeft(node, rbound)
+          )
+        }
+      )
+      case Some(lbound) => (
+        match rbound {
+          case None => (
+            CutoffNodeAndKeepRight(node, lbound)
+          )
+          case Some(rbound) => (
+            var node1 := CutoffNodeAndKeepLeft(node, rbound);
+            CutoffNodeAndKeepLeftCorrect(node, rbound); // we need WFNode(node1)
+            CutoffNodeAndKeepRight(node1, lbound)
+          )
+        }
+      )
+    }
+  }
+
+  lemma CutoffNodeCorrect(node: Node, lbound: Option<Key>, rbound: Option<Key>)
+  requires WFNode(node)
+  requires BT.WFNode(INode(node))
+  ensures var node' := CutoffNode(node, lbound, rbound);
+    && WFNode(node')
+    && INode(node') == BT.CutoffNode(INode(node), lbound, rbound)
+  {
+    reveal_CutoffNode();
+    BT.reveal_CutoffNode();
+
+    match lbound {
+      case None => {
+        match rbound {
+          case None => {
+          }
+          case Some(rbound) => {
+            CutoffNodeAndKeepLeftCorrect(node, rbound);
+          }
+        }
+      }
+      case Some(lbound) => {
+        match rbound {
+          case None => {
+            CutoffNodeAndKeepRightCorrect(node, lbound);
+          }
+          case Some(rbound) => {
+            var node1 := CutoffNodeAndKeepLeft(node, rbound);
+            CutoffNodeAndKeepLeftCorrect(node, rbound);
+            CutoffNodeAndKeepRightCorrect(node1, lbound);
+          }
+        }
+      }
+    }
+  }
+
+  function method {:opaque} SplitChildLeft(child: Node, num_children_left: int) : Node
+  requires 0 <= num_children_left - 1 <= |child.pivotTable|
+  requires child.children.Some? ==> 0 <= num_children_left <= |child.children.value|
+  requires 0 <= num_children_left <= |child.buckets|
+  {
+    Node(
+      child.pivotTable[ .. num_children_left - 1 ],
+      if child.children.Some? then Some(child.children.value[ .. num_children_left ]) else None,
+      child.buckets[ .. num_children_left ]
+    )
+  }
+
+  function method {:opaque} SplitChildRight(child: Node, num_children_left: int) : Node
+  requires 0 <= num_children_left <= |child.pivotTable|
+  requires child.children.Some? ==> 0 <= num_children_left <= |child.children.value|
+  requires 0 <= num_children_left <= |child.buckets|
+  {
+    Node(
+      child.pivotTable[ num_children_left .. ],
+      if child.children.Some? then Some(child.children.value[ num_children_left .. ]) else None,
+      child.buckets[ num_children_left .. ]
+    )
+  }
+
+  lemma lemmaSplitChild(child: Node, num_children_left: int)
+  requires WFNode(child)
+  requires BT.WFNode(INode(child))
+  requires 1 <= num_children_left <= |child.buckets| - 1
+  ensures WFNode(SplitChildLeft(child, num_children_left))
+  ensures WFNode(SplitChildRight(child, num_children_left))
+  ensures INode(SplitChildLeft(child, num_children_left)) == BT.SplitChildLeft(INode(child), num_children_left)
+  ensures INode(SplitChildRight(child, num_children_left)) == BT.SplitChildRight(INode(child), num_children_left)
+  {
+    reveal_SplitChildLeft();
+    reveal_SplitChildRight();
+    Pivots.WFSlice(child.pivotTable, 0, num_children_left - 1);
+    Pivots.WFSuffix(child.pivotTable, num_children_left);
+    KMTable.Islice(child.buckets, 0, num_children_left);
+    KMTable.Isuffix(child.buckets, num_children_left);
+    WFBucketListSplitLeft(KMTable.ISeq(child.buckets), child.pivotTable, num_children_left);
+    WFBucketListSplitRight(KMTable.ISeq(child.buckets), child.pivotTable, num_children_left);
+    assert WFNode(SplitChildRight(child, num_children_left));
+    assert WFNode(SplitChildLeft(child, num_children_left));
+  }
+
+  // TODO can we get BetreeBlockCache to ensure that will be true generally whenever taking a betree step?
+  // This sort of proof logic shouldn't have to be in the implementation.
+  lemma lemmaSplitChildValidReferences(child1: BT.G.Node, child: BT.G.Node, num_children_left: int, graph: map<BT.G.Reference, seq<BT.G.Reference>>, lbound: Option<Key>, rbound: Option<Key>)
+  requires BT.WFNode(child1)
+  requires BT.WFNode(child)
+  requires 1 <= num_children_left <= |child.buckets| - 1
+  requires BC.BlockPointsToValidReferences(child1, graph);
+  requires child == BT.CutoffNode(child1, lbound, rbound);
+  ensures BC.BlockPointsToValidReferences(BT.SplitChildLeft(child, num_children_left), graph);
+  ensures BC.BlockPointsToValidReferences(BT.SplitChildRight(child, num_children_left), graph);
+  {
+  }
+
+  function SplitParent(fused_parent: Node, pivot: Key, slot_idx: int, left_childref: BT.G.Reference, right_childref: BT.G.Reference)
+  : (res : Node)
+  requires WFNode(fused_parent)
+  requires 0 <= slot_idx < |fused_parent.buckets|
+  requires fused_parent.children.Some?
+  {
+    var pivots := Sequences.insert(fused_parent.pivotTable, pivot, slot_idx);
+    var buckets := KMTable.splitKMTableInList(fused_parent.buckets, slot_idx, pivot);
+    Node(
+      pivots,
+      Some(replace1with2(fused_parent.children.value, left_childref, right_childref, slot_idx)),
+      buckets
+    )
+  }
+
+  lemma SplitParentCorrect(fused_parent: Node, pivot: Key, slot_idx: int, left_childref: BT.G.Reference, right_childref: BT.G.Reference)
+  requires WFNode(fused_parent)
+  requires BT.WFNode(INode(fused_parent))
+  requires 0 <= slot_idx < |fused_parent.buckets|
+  requires PivotsLib.PivotInsertable(fused_parent.pivotTable, slot_idx, pivot)
+  requires fused_parent.children.Some?
+  ensures var res := SplitParent(fused_parent, pivot, slot_idx, left_childref, right_childref);
+    && WFNode(res)
+    && INode(res) == BT.SplitParent(INode(fused_parent), pivot, slot_idx, left_childref, right_childref)
+  {
+    KMTable.splitKMTableInListCorrect(fused_parent.buckets, slot_idx, pivot);
+    var res := SplitParent(fused_parent, pivot, slot_idx, left_childref, right_childref);
+    WFSplitBucketInList(KMTable.ISeq(fused_parent.buckets), slot_idx, pivot, fused_parent.pivotTable);
+    assert WFNode(res);
+    assert INode(res) == BT.SplitParent(INode(fused_parent), pivot, slot_idx, left_childref, right_childref);
+  }
+
+  lemma lemmaSplitParentValidReferences(fused_parent: BT.G.Node, pivot: Key, slot_idx: int, left_childref: BT.G.Reference, right_childref: BT.G.Reference, graph: map<BT.G.Reference, seq<BT.G.Reference>>)
+  requires BT.WFNode(fused_parent)
+  requires 0 <= slot_idx < |fused_parent.buckets|
+  requires fused_parent.children.Some?
+  requires BC.BlockPointsToValidReferences(fused_parent, graph);
+  requires left_childref in graph
+  requires right_childref in graph
+  ensures BC.BlockPointsToValidReferences(BT.SplitParent(fused_parent, pivot, slot_idx, left_childref, right_childref), graph);
+  {
+    var split_parent := BT.SplitParent(fused_parent, pivot, slot_idx, left_childref, right_childref);
+    forall r | r in BT.G.Successors(split_parent)
+    ensures r in graph
+    {
+      assert BC.BlockPointsToValidReferences(fused_parent, graph);
+      var idx :| 0 <= idx < |split_parent.children.value| && split_parent.children.value[idx] == r;
+      if (idx < slot_idx) {
+        assert r == fused_parent.children.value[idx];
+        assert r in graph;
+      } else if (idx == slot_idx) {
+        assert r == left_childref;
+        assert r in graph;
+      } else if (idx == slot_idx + 1) {
+        assert r == right_childref;
+        assert r in graph;
+      } else {
+        assert r == fused_parent.children.value[idx-1];
+        assert r in graph;
+      }
+    }
+  }
+
+  function {:opaque} doSplit(k: Constants, s: Variables, parentref: BT.G.Reference, ref: BT.G.Reference, slot: int)
+  : (s': Variables)
+  requires s.Ready?
+  requires Inv(k, s)
+  requires ref in s.ephemeralIndirectionTable
+  requires parentref in s.ephemeralIndirectionTable
+  requires ref in s.cache
+  requires parentref in s.cache
+  requires s.cache[parentref].children.Some?
+  requires 0 <= slot < |s.cache[parentref].children.value|
+  requires s.cache[parentref].children.value[slot] == ref
+  {
+    if (
+      && s.frozenIndirectionTable.Some?
+      && parentref in s.frozenIndirectionTable.value
+      && var entry := s.frozenIndirectionTable.value[parentref];
+      && var (loc, _) := entry;
+      && loc.None?
+    ) then (
+      s
+    ) else (
+      var fused_parent := s.cache[parentref];
+      var fused_child := s.cache[ref];
+
+      var lbound := (if slot > 0 then Some(fused_parent.pivotTable[slot - 1]) else None);
+      var ubound := (if slot < |fused_parent.pivotTable| then Some(fused_parent.pivotTable[slot]) else None);
+      var child := CutoffNode(fused_child, lbound, ubound);
+
+      if (|child.pivotTable| == 0) then (
+        // TODO there should be an operation which just
+        // cuts off the node and doesn't split it.
+        s
+      ) else (
+        var left_childref := getFreeRef(s);
+        if left_childref.None? then (
+          s
+        ) else (
+          var right_childref := getFreeRef2(s, left_childref.value);
+          if right_childref.None? then (
+            s
+          ) else (
+            var num_children_left := |child.buckets| / 2;
+            var pivot := child.pivotTable[num_children_left - 1];
+
+            var left_child := SplitChildLeft(child, num_children_left);
+            var right_child := SplitChildRight(child, num_children_left);
+            var split_parent := SplitParent(fused_parent, pivot, slot, left_childref.value, right_childref.value);
+
+            var s1 := write(k, s, left_childref.value, left_child);
+            var s2 := write(k, s1, right_childref.value, right_child);
+            var s' := write(k, s2, parentref, split_parent);
+            s'
+          )
+        )
+      )
+    )
+  }
+
+  lemma doSplitCorrect(k: Constants, s: Variables, parentref: BT.G.Reference, ref: BT.G.Reference, slot: int)
+  requires s.Ready?
+  requires Inv(k, s)
+  requires ref in s.ephemeralIndirectionTable
+  requires parentref in s.ephemeralIndirectionTable
+  requires ref in s.cache
+  requires parentref in s.cache
+  requires s.cache[parentref].children.Some?
+  requires 0 <= slot < |s.cache[parentref].children.value|
+  requires s.cache[parentref].children.value[slot] == ref
+  requires s.rootBucket == map[] // FIXME we don't actually need this unless paretnref is root
+  ensures var s' := doSplit(k, s, parentref, ref, slot);
+    && WFVars(s')
+    && M.Next(Ik(k), IVars(s), IVars(s'), UI.NoOp, D.NoDiskOp)
+  {
+    reveal_doSplit();
+
+    if (
+      && s.frozenIndirectionTable.Some?
+      && parentref in s.frozenIndirectionTable.value
+      && var entry := s.frozenIndirectionTable.value[parentref];
+      && var (loc, _) := entry;
+      && loc.None?
+    ) {
+      assert noop(k, IVars(s), IVars(s));
+    } else {
+      var fused_parent := s.cache[parentref];
+      var fused_child := s.cache[ref];
+
+      INodeRootEqINodeForEmptyRootBucket(fused_parent);
+      INodeRootEqINodeForEmptyRootBucket(fused_child);
+
+      var lbound := (if slot > 0 then Some(fused_parent.pivotTable[slot - 1]) else None);
+      var ubound := (if slot < |fused_parent.pivotTable| then Some(fused_parent.pivotTable[slot]) else None);
+      var child := CutoffNode(fused_child, lbound, ubound);
+      CutoffNodeCorrect(fused_child, lbound, ubound);
+
+      if (|child.pivotTable| == 0) {
+        // TODO there should be an operation which just
+        // cuts off the node and doesn't split it.
+        assert noop(k, IVars(s), IVars(s));
+      } else {
+        var left_childref := getFreeRef(s);
+        if left_childref.None? {
+          assert noop(k, IVars(s), IVars(s));
+        } else {
+          var right_childref := getFreeRef2(s, left_childref.value);
+          if right_childref.None? {
+            assert noop(k, IVars(s), IVars(s));
+          } else {
+            var num_children_left := |child.buckets| / 2;
+            var pivot := child.pivotTable[num_children_left - 1];
+            PivotsLib.PivotNotMinimum(child.pivotTable, num_children_left - 1);
+
+            var left_child := SplitChildLeft(child, num_children_left);
+            var right_child := SplitChildRight(child, num_children_left);
+            var split_parent := SplitParent(fused_parent, pivot, slot, left_childref.value, right_childref.value);
+
+            reveal_write();
+            var s1 := write(k, s, left_childref.value, left_child);
+            var s2 := write(k, s1, right_childref.value, right_child);
+            var s' := write(k, s2, parentref, split_parent);
+
+            lemmaSplitChild(child, num_children_left);
+            SplitParentCorrect(fused_parent, pivot, slot, left_childref.value, right_childref.value);
+
+            lemmaBlockPointsToValidReferences(k, s, ref);
+            assert BC.BlockPointsToValidReferences(INode(fused_child), IIndirectionTable(s.ephemeralIndirectionTable).graph);
+            lemmaSplitChildValidReferences(INode(fused_child), INode(child), num_children_left, IIndirectionTable(s.ephemeralIndirectionTable).graph, lbound, ubound);
+
+            writeNewRefIsAlloc(k, s, left_childref.value, left_child);
+            writeNewRefIsAlloc(k, s1, right_childref.value, right_child);
+
+            lemmaBlockPointsToValidReferences(k, s, parentref);
+            assert BC.BlockPointsToValidReferences(INode(fused_parent), IIndirectionTable(s2.ephemeralIndirectionTable).graph);
+            lemmaSplitParentValidReferences(INode(fused_parent), pivot, slot, left_childref.value, right_childref.value, IIndirectionTable(s2.ephemeralIndirectionTable).graph);
+
+            writeCorrect(k, s2, parentref, split_parent);
+          
+            reveal_SplitChildLeft();
+            reveal_SplitChildRight();
+
+            assert WFBuckets(child.buckets);
+            assert INode(child) == BT.CutoffNode(INode(fused_child), lbound, ubound);
+            assert 1 <= num_children_left < |child.buckets|;
+
+            var splitStep := BT.NodeFusion(
+              parentref,
+              ref,
+              left_childref.value,
+              right_childref.value,
+              INode(fused_parent),
+              INode(split_parent),
+              INode(fused_child),
+              INode(left_child),
+              INode(right_child),
+              slot,
+              num_children_left,
+              pivot
+            );
+
+            assert splitStep.num_children_left == num_children_left;
+            assert splitStep.fused_child == INode(fused_child);
+
+            assert left_childref.value != right_childref.value;
+            assert BT.ValidSplit(splitStep);
+            var step := BT.BetreeSplit(splitStep);
+            ghost var ops := [
+              BT.G.AllocOp(left_childref.value, INode(left_child)),
+              BT.G.AllocOp(right_childref.value, INode(right_child)),
+              BT.G.WriteOp(parentref, INode(split_parent))
+            ];
+            assert ops == BT.BetreeStepOps(step);
+            BC.MakeTransaction3(Ik(k), IVars(s), IVars(s1), IVars(s2), IVars(s'), ops);
+            assert stepsBetree(k, IVars(s), IVars(s'), UI.NoOp, step);
+          }
+        }
+      }
+    }
+  }
+}
